experiment/Experiment.Steel.fsti
@@ -1,0 +1,243 @@
+module Experiment.Steel
+
+/// Interface for the functionalisation of Steel programs
+
+module U    = Learn.Util
+module L    = FStar.List.Pure
+module SE   = Steel.Effect
+module Ll   = Learn.List
+module Dl   = Learn.DList
+module Fl   = Learn.FList
+module Perm = Learn.Permutation
+
+module M    = Experiment.Steel.Repr.M
+module ST   = Experiment.Steel.Repr.ST
+module SF   = Experiment.Steel.Repr.SF
+module Fun  = Experiment.Repr.Fun
+module CSl  = Experiment.Steel.CondSolver
+
+open FStar.Tactics
+open Learn.Tactics.Util
+
+
+let prog_M_to_Fun
+      (#a : Type) (t : M.repr a)
+      (#pre : M.pre_t) (#post : M.post_t a)
+      (c : M.prog_cond t.repr_tree pre post)
+  : (sl0 : M.sl_t pre) ->
+    Fun.prog_tree #SF.sl_tys SF.({val_t = a; sel_t = ST.post_ST_of_M post})
+  =
+    let (|t_M, s_M|) = c in
+    let t_ST    = ST.repr_ST_of_M t.repr_tree t_M   in
+    let shp_ST  = ST.shape_ST_of_M s_M.shp          in
+    (**) ST.repr_ST_of_M_shape t.repr_tree t_M s_M.shp;
+    let t_ST'   = ST.flatten_prog t_ST              in
+    let shp_ST' = ST.flatten_shape shp_ST           in
+    (**) ST.flatten_prog_shape t_ST shp_ST;
+    let s_ST'   = ST.mk_prog_shape t_ST' shp_ST'    in
+    begin fun (sl0 : M.sl_t pre) ->
+      let t_SF = SF.repr_SF_of_ST_rall t_ST' s_ST' sl0 in
+      SF.repr_Fun_of_SF t_SF
+    end
+
+val prog_M_to_Fun_equiv
+      (#a : Type) (t : M.repr a)
+      (#pre : M.pre_t) (#post : M.post_t a)
+      (c : M.prog_cond t.repr_tree pre post)
+      (sl0 : M.sl_t pre)
+  : Lemma (M.tree_req t.repr_tree c._1 sl0 <==> Fun.tree_req (prog_M_to_Fun t c sl0) /\
+          (M.tree_req t.repr_tree c._1 sl0 ==>
+          (forall (x : a) (sl1 : M.sl_t (post x)) .
+               (M.tree_ens t.repr_tree c._1 sl0 x sl1 <==>
+                Fun.tree_ens (prog_M_to_Fun t c sl0) SF.({val_v = x; sel_v = sl1})))))
+
+inline_for_extraction
+val prog_M_to_Fun_extract
+      (#a : Type) (t : M.repr a)
+      (#pre : M.pre_t) (#post : M.post_t a)
+      (c : M.prog_cond t.repr_tree pre post)
+      (req : M.req_t pre) (ens : M.ens_t pre a post)
+      (sub : (sl0 : M.sl_t pre) -> Lemma (requires req sl0)
+               (ensures Fun.tree_req (prog_M_to_Fun t c sl0) /\
+                  (forall (x : a) (sl1 : M.sl_t (post x)) .
+                    Fun.tree_ens (prog_M_to_Fun t c sl0) SF.({val_v = x; sel_v = sl1}) ==> ens sl0 x sl1)))
+  : M.repr_steel_t a pre post req ens
+
+inline_for_extraction
+val prog_M_to_Fun_extract_wp
+      (#a : Type) (t : M.repr a)
+      (#pre : M.pre_t) (#post : M.post_t a)
+      (c : M.prog_cond t.repr_tree pre post)
+      (req : M.req_t pre) (ens : M.ens_t pre a post)
+      (wp : (sl0 : M.sl_t pre) -> Lemma
+              (Fun.tree_wp (prog_M_to_Fun t c sl0) (fun res -> ens sl0 res.val_v res.sel_v)))
+  : M.repr_steel_t a pre post req ens
+
+
+
+let __normal_M : list norm_step = [
+  delta_only [`%M.vprop_list_sels_t;      `%M.Mkrepr?.repr_tree;
+              `%M.Mkprog_shape?.post_len; `%M.Mkprog_shape?.shp;
+              `%L.map; `%SE.Mkvprop'?.t;
+              `%prog_M_to_Fun];
+  delta_attr [`%__tac_helper__; `%M.__repr_M__;
+              `%SE.__steel_reduce__; `%SE.__reduce__];
+  delta_qualifier ["unfold"];
+  iota; zeta
+]
+
+let __normal_ST : list norm_step = [
+  delta_only [`%ST.repr_ST_of_M; `%ST.bind; `%ST.post_ST_of_M;
+              `%M.vprop_list_sels_t; `%L.map; `%SE.Mkvprop'?.t;
+              `%ST.const_post; `%ST.frame_post; `%L.op_At; `%L.append;
+              `%ST.flatten_prog; `%ST.flatten_prog_aux; `%ST.flatten_prog_k_id;
+
+              `%ST.shape_ST_of_M; `%ST.flatten_shape; `%ST.flatten_shape_aux; `%ST.flatten_shape_k_id;
+              `%M.Mkprog_shape?.post_len; `%M.Mkprog_shape?.shp;
+              `%Perm.perm_f_to_list; `%Ll.initi; `%Perm.id_n; `%Perm.mk_perm_f;
+              `%M.Mkprog_shape?.post_len; `%M.Mkprog_shape?.shp];
+  delta_qualifier ["unfold"];
+  delta_attr [`%SE.__steel_reduce__];
+  iota; zeta; primops
+]
+
+let __normal_SF : list norm_step = [
+  delta_only [`%SF.repr_SF_of_ST_rall; `%SF.repr_SF_of_ST; `%SF.shape_SF_of_ST; `%SF.shape_SF_of_ST_rall;
+              `%SF.post_SF_of_ST; `%SF.postl_SF_of_ST; `%SF.post_bij;
+              `%ST.Mkprog_shape?.post_len; `%ST.Mkprog_shape?.shp;
+              `%SF.Mkpost_bij_t'?.len_SF; `%SF.Mkpost_bij_t'?.idx_SF; `%SF.Mkpost_bij_t'?.idx_ST;
+              `%Ll.initi; `%L.index; `%L.hd; `%L.tl; `%L.tail; `%L.length;
+              `%SF.sel_ST_of_SF; `%SF.sell_ST_of_SF; `%SF.post_src_of_shape;
+              `%SF.post_src_f_of_shape; `%SF.sel_SF_of_ST; `%SF.sell_SF_of_ST;
+              `%Fl.splitAt_ty; `%Fl.head; `%Fl.tail;
+              `%Fl.dlist_of_f; `%Dl.initi; `%Fl.cons; `%Fl.nil;
+              `%Mktuple2?._1;`%Mktuple2?._2;
+              `%Learn.Option.map;
+              `%Perm.perm_f_swap; `%Perm.perm_f_transpose; `%Perm.perm_f_of_pair;
+              `%Perm.mk_perm_f; `%Perm.id_n; `%Perm.perm_f_of_list];
+  delta_qualifier ["unfold"];
+  delta_attr [`%U.__util_func__];
+  iota; zeta; primops
+]
+
+let __normal_Fun : list norm_step = [
+  delta_only [`%SF.repr_Fun_of_SF;
+              `%SF.shape_Fun_of_SF; `%SF.Mkprog_shape?.post_len; `%SF.Mkprog_shape?.shp];
+  delta_qualifier ["unfold"];
+  iota; zeta; primops
+]
+
+let __normal_Fun_elim_returns_0 : list norm_step = [
+  delta_only [`%Fun.elim_returns; `%Fun.elim_returns_aux; `%Fun.elim_returns_k_trm; `%Fun.elim_returns_k_ret;
+              `%SF.sl_tys; `%SF.sl_tys_lam;
+              `%Fun.Mktys'?.v_of_r; `%Fun.Mktys'?.r_of_v;
+              `%Fun.Mktys_lam'?.lam_prop; `%Fun.Mktys_lam'?.lam_tree;
+              `%SF.Mksl_tys_t?.val_t;     `%SF.Mksl_tys_t?.sel_t;
+              `%SF.Mksl_tys_v?.val_v;     `%SF.Mksl_tys_v?.sel_v;
+              `%SF.Mksl_tys_r?.vl;        `%SF.Mksl_tys_r?.sl;
+              `%Fun.Tret?.x;
+              `%SF.sl_r_of_v; `%SF.sl_v_of_r;
+              `%Fl.cons; `%Fl.nil; `%Fl.dlist_of_f; `%Fl.flist_of_d'; `%Dl.initi; `%Dl.index;
+              `%L.length; `%L.index; `%L.hd; `%L.tl; `%L.tail; `%Ll.initi
+              ];
+  delta_qualifier ["unfold"];
+  iota; zeta; primops
+]
+
+let __normal_Fun_elim_returns_1 : list norm_step = [
+  delta_only [`%SF.delayed_sl_uncurrify];
+  delta_qualifier ["unfold"];
+  iota; zeta; primops
+]
+
+let __normal_Fun_spec : list norm_step = [
+  delta_only [`%Fun.tree_wp; `%Fl.partial_app_flist;
+              `%Fun.Mktys'?.all; `%SF.sl_tys; `%SF.sl_all; `%Fl.forall_flist;
+              `%Fun.Mktys'?.v_of_r; `%SF.sl_v_of_r; `%Fl.flist_of_d';
+              `%Fl.cons; `%Fl.nil;
+              `%SF.Mksl_tys_t?.val_t; `%SF.Mksl_tys_t?.sel_t;
+              `%SF.Mksl_tys_v?.val_v; `%SF.Mksl_tys_v?.sel_v;
+              `%SF.Mksl_tys_r?.vl; `%SF.Mksl_tys_r?.sl];
+  delta_qualifier ["unfold"];
+  delta_attr [`%SE.__steel_reduce__];
+  iota; zeta; primops
+]
+
+let __normal_vprop_list : list norm_step = [
+  delta_only [`%M.rmem_sels; `%Fl.flist_of_d; `%M.rmem_sl_list; `%M.vpl_sels;
+              `%Dl.index; `%L.length; `%L.index; `%Fl.flist];
+  delta_attr [`%SE.__reduce__];
+  iota; zeta;
+]
+
+
+(***** Calling a [M.repr_steel_t] from a Steel program *)
+
+unfold
+let norm_vpl (#a : Type) (x : a) = Pervasives.norm __normal_vprop_list x
+
+inline_for_extraction
+val call_repr_steel
+      (#a : Type)
+      (#pre : M.pre_t)     (#post : M.post_t a)
+      (#req : M.req_t pre) (#ens  : M.ens_t pre a post)
+      (r : M.repr_steel_t a pre post req ens)
+  : SE.Steel a (M.vprop_of_list pre) (fun x -> M.vprop_of_list (post x))
+      (requires fun h0      -> req (norm_vpl (M.rmem_sels pre h0)))
+      (ensures  fun h0 x h1 -> ens (norm_vpl (M.rmem_sels pre h0))
+                                x
+                                (norm_vpl (M.rmem_sels (post x) h1)))
+
+
+(***** Extracting a [M.repr_steel_t] from a [M.repr] *)
+
+/// We mention [t] so that it is specified by the goal, but this type is just a synonym for [M.repr_steel_t].
+let extract (a : Type) (pre : M.pre_t) (post : M.post_t a) (req : M.req_t pre) (ens : M.ens_t pre a post)
+            (t : M.repr a)
+  : Type
+  = M.repr_steel_t a pre post req ens
+
+
+inline_for_extraction
+let __solve_by_wp
+      (#a : Type) (#t : M.repr a)
+      (#pre : M.pre_t) (#post : M.post_t a)
+      (#req : M.req_t pre) (#ens : M.ens_t pre a post)
+      (c : M.prog_cond t.repr_tree pre post)
+      (t_Fun : (sl0 : M.sl_t pre) -> Fun.prog_tree #SF.sl_tys SF.({val_t = a; sel_t = ST.post_ST_of_M post}))
+      (t_Fun_eq : squash (t_Fun == (fun sl0 -> prog_M_to_Fun t c sl0)))
+      (wp : squash (Fl.forall_flist (M.vprop_list_sels_t pre) (fun sl0 ->
+               Fun.tree_wp (t_Fun sl0) (fun res -> ens sl0 res.val_v res.sel_v))))
+  : extract a pre post req ens t
+  =
+    prog_M_to_Fun_extract_wp t c req ens (fun sl0 -> ())
+
+let solve_by_wp () : Tac unit
+  =
+    let u_c = fresh_uvar None in
+    let u_t_Fun = fresh_uvar None in
+    apply_raw (`(__solve_by_wp (`#u_c) (`#u_t_Fun)));
+
+    let t = timer_start   "prog_cond " in
+    unshelve u_c;
+    norm __normal_M;
+    CSl.build_prog_cond ();
+
+    (* TODO? stage prog_M_to_Fun to avoid duplication *)
+    let t = timer_enter t "normal_M  " in
+    norm __normal_M;
+    let t = timer_enter t "normal_ST " in
+    norm __normal_ST;
+    let t = timer_enter t "normal_SF " in
+    norm __normal_SF;
+    let t = timer_enter t "normal_Fun" in
+    norm __normal_Fun;
+    let t = timer_enter t "misc      " in
+    trefl ();
+
+    (* wp *)
+    let t = timer_enter t "Fun_wp    " in
+    norm __normal_M;
+    norm __normal_Fun_spec;
+    timer_stop t;
+    smt ()
